Changed name of Tokeneer2 to Tokeneer and removed unnecessary files

LAB2/Tokeneer/Tokeneer.dfy
@@ -1,3 +1,29 @@
+/*
+While the real system has a very large specification, this question asks you to model a 
+high-level mini-version of the Tokeneer system in Dafny and verify its correctness. 
+
+The picture below shows the secure door system you are to model and verify. 
+
+To enter the door,
+*********** the user first needs to enrol and receive a token <--- TODO (1) ******************, which stores fingerprint data (for 
+ simplicity, you may assume fingerprints are represented by integers) and the security clearance 
+ level (there are three clearance levels: Low, Medium and High). 
+
+ ************* The enrolment station keeps track of the users in the system to make sure no one can be issued with more than one token at the time. <--- TODO (2) *******************
+
+When a user wants to open a door, the ID station checks that the user's fingerprint agrees with 
+what is stored on the user's token and that the user have the adequate security clearance to enter 
+this door. 
+
+If a security breach is discovered, i.e. a token is used by the wrong person, this token 
+must be invalidated immediately and ************* the alarm sound. (3) <--- TODO ***********
+*/
+
+// Defined clearance levels
+static function method HIGH(): int {3} 
+static function method MEDIUM(): int {2}
+static function method LOW(): int {1}
+
 class Token {
 	var fingerprint : int;
 	var clearanceLevel : int;
@@ -5,45 +31,36 @@ class Token {
 	
 	method Init(fingerprint : int, clearanceLevel : int)
 	modifies this;
+	requires clearanceLevel == HIGH() || clearanceLevel == MEDIUM() || clearanceLevel == LOW();
 	ensures this.fingerprint == fingerprint && this.clearanceLevel == clearanceLevel && valid == true;
 	{
 		this.fingerprint := fingerprint;
 		this.clearanceLevel := clearanceLevel;
 		valid := true;
 	}
-	
-	function method ValidateFingerPrint(scannedFingerprint : int) : bool
-	reads this;
-	{
-		fingerprint == scannedFingerprint
-	}
 }
 
-class Door {
+class Door { // Aka ID Station
 	var requiredClearanceLevel : int;
-
-	static function method HIGH(): int {3} 
-	static function method MEDIUM(): int {2}
-	static function method LOW(): int {1}
 	
 	method Init(requiredClearanceLevel : int)
 	modifies this;
+	requires requiredClearanceLevel == HIGH() || requiredClearanceLevel == MEDIUM() || requiredClearanceLevel == LOW();
 	ensures this.requiredClearanceLevel == requiredClearanceLevel;
 	{
 		this.requiredClearanceLevel := requiredClearanceLevel;
 	}
 	
-	method EnterDoor(user : User) returns (accessGranted : bool)
+	method EnterDoor(user : User, fingerPrint : int) returns (accessGranted : bool)
 	modifies user.token`valid;
 	requires user != null && user.token != null;
-	ensures user.token.valid && user.token.ValidateFingerPrint(user.ScanFinger()) && ValidateClearanceLevel(user.token) ==> accessGranted && user.token.valid;
-	ensures !user.token.valid ==> !accessGranted && !user.token.valid;
-	ensures !user.token.ValidateFingerPrint(user.ScanFinger()) ==> !accessGranted && !user.token.valid;
-	ensures !ValidateClearanceLevel(user.token) ==> !accessGranted;
+	ensures !old(user.token.valid) || !ValidateFingerPrint(user.token, fingerPrint) ==> !accessGranted && !user.token.valid;
+	ensures old(user.token.valid) && ValidateFingerPrint(user.token, fingerPrint) && ValidateClearanceLevel(user.token) ==> accessGranted && user.token.valid;
+	ensures old(user.token.valid) && ValidateFingerPrint(user.token, fingerPrint) && !ValidateClearanceLevel(user.token) ==> !accessGranted && user.token.valid;
 	{
 		if (user.token.valid)
 		{
-			var validFingerPrint := user.token.ValidateFingerPrint(user.ScanFinger());
+			var validFingerPrint := ValidateFingerPrint(user.token, fingerPrint);
 			if (!validFingerPrint)
 			{
 				user.token.valid := false;
@@ -64,91 +81,207 @@ class Door {
 	{
 		token.clearanceLevel >= requiredClearanceLevel
 	}
+
+	function method ValidateFingerPrint(token : Token, scannedFingerprint : int) : bool
+	reads token;
+	requires token != null;
+	{
+		token.fingerprint == scannedFingerprint
+	}
 }
 
 class User {
 	var token : Token;
-	var fingerprint : int;
 	
-	method Init(fingerprint : int, token: Token)
+	method Init()
 	modifies this;
-	requires token != null;
-	ensures this.fingerprint == fingerprint && this.token == token;
+	ensures this.token == null;
 	{
-		this.fingerprint := fingerprint;
-		this.token := token;
+		this.token := null;
 	}
-	
-	function method ScanFinger() : int
-	reads this;
-	{
-		fingerprint
-	}
+
 }
 
 class EnrolmentStation {
-	var users : set<User>; //behövs denna??
-	
-	method PrintAccess(accessGranted : bool, tokenValid : bool)
+	var users : set<User>; //behövs denna?? Svar: Ja, för enrolment. kolla (1) och (2) i specifikationen överst 
+
+	method Init()
+	modifies this;
+	ensures users == {};
+	ensures fresh(users);
 	{
-		if (accessGranted)
-			{
-				print "Access granted!\n\n";
-			}
-			else
-			{
-				print "Access denied!\n";
-			if (!tokenValid)
-			{
-				print "Token invalid!\n\n";
-			}
-			else
-			{
-				print "\n";
-			}
-		}
+		users := {};
 	}
 	
-	method Main()
+	//  löser både (1) och (2) i specc.
+	method Enrol(user : User, clearanceLevel : int, fingerPrint : int) 
+	modifies this, user`token, user.token;
+	requires user != null && user.token == null;
+	requires clearanceLevel == HIGH() || clearanceLevel == MEDIUM() || clearanceLevel == LOW();
+	requires user !in users; 
+	ensures users == old(users) + {user}; 
+	ensures user.token != null; 
+	ensures user.token.fingerprint == fingerPrint;
+	ensures user.token.clearanceLevel == clearanceLevel;
+	ensures user.token.valid == true;
+	ensures fresh(user.token);
 	{
-		var clearanceLevelHigh := 3;
-		var clearanceLevelMedium := 2;
-		var clearanceLevelLow := 1;
-		
-		var token1 := new Token.Init(1, clearanceLevelHigh);
-		var door1 := new Door.Init(clearanceLevelHigh);
-		var enrolmentStation := new EnrolmentStation;
-		
-		var user1 := new User.Init(1, token1);
-		var accessGranted := door1.EnterDoor(user1);
-		print "user1 with correct fingerprint tries to access door1 with token1 (Clearance level enough):\n";
-		PrintAccess(accessGranted, token1.valid);
-		
-		var user2 := new User.Init(2, token1);
-		accessGranted := door1.EnterDoor(user2);
-		print "user2 with wrong fingerprint tries to access door1 with token1 (Clearance level enough):\n";
-		PrintAccess(accessGranted, token1.valid);
-		
-		var user3 := new User.Init(1, token1);
-		accessGranted := door1.EnterDoor(user3);
-		print "user3 with correct fingerprint tries to access door1 with token1 again with invalid token (Clearance level enough):\n";
-		PrintAccess(accessGranted, token1.valid);
-		
-		var token2 := new Token.Init(1, clearanceLevelMedium);
-		
-		var user4 := new User.Init(1, token2);
-		accessGranted := door1.EnterDoor(user4);
-		print "user4 with correct fingerprint tries to access door1 with token2 (Clearance level to low):\n";
-		PrintAccess(accessGranted, token2.valid);
-		
-		var door2 := new Door.Init(clearanceLevelMedium);
-		accessGranted := door2.EnterDoor(user4);
-		print "user4 with correct fingerprint tries to access door2 with token2 (Clearance level enough):\n";
-		PrintAccess(accessGranted, token2.valid);
-		
-		var door3 := new Door.Init(clearanceLevelLow);
-		accessGranted := door3.EnterDoor(user4);
-		print "user4 with correct fingerprint tries to access door3 with token2 (Clearance level more than needed):\n";
-		PrintAccess(accessGranted, token2.valid);
+		user.token := new Token.Init(fingerPrint, clearanceLevel);
+		users := users + {user};
 	}
+}
+
+method Main() // TODO ska nog använda asserts här istället för prints som i excercises
+{
+		// Enrolment station
+		var enrolmentStation := new EnrolmentStation.Init();
+
+		// Doors
+		var doorHigh := new Door.Init(HIGH());
+		var doorMedium := new Door.Init(MEDIUM());
+		var doorLow := new Door.Init(LOW());
+
+		// Users
+		var userHigh1 := new User.Init();
+	    var userHigh2 := new User.Init();
+		var userMedium3 := new User.Init();
+	    var userMedium4 := new User.Init();
+	    var userLow5 := new User.Init();
+	    var userLow6 := new User.Init();
+
+
+		// ******* Enrolment tests *******
+		enrolmentStation.Enrol(userHigh1, HIGH(), 1);
+
+		assert enrolmentStation.users == {userHigh1};
+		assert userHigh1.token.clearanceLevel == HIGH();
+		assert userHigh1.token.fingerprint == 1;
+		assert userHigh1.token.valid;
+
+		enrolmentStation.Enrol(userHigh2, HIGH(), 2);
+
+		assert enrolmentStation.users == {userHigh1, userHigh2};
+		assert userHigh2.token.clearanceLevel == HIGH();
+		assert userHigh2.token.fingerprint == 2;
+		assert userHigh2.token.valid;
+
+		enrolmentStation.Enrol(userMedium3, MEDIUM(), 3);
+
+		assert enrolmentStation.users == {userHigh1, userHigh2, userMedium3};
+		assert userMedium3.token.clearanceLevel == MEDIUM();
+		assert userMedium3.token.fingerprint == 3;
+		assert userMedium3.token.valid;
+
+		enrolmentStation.Enrol(userMedium4, MEDIUM(), 4);
+
+		assert enrolmentStation.users == {userHigh1, userHigh2, userMedium3, userMedium4};
+		assert userMedium4.token.clearanceLevel == MEDIUM();
+		assert userMedium4.token.fingerprint == 4;
+		assert userMedium4.token.valid;
+
+		enrolmentStation.Enrol(userLow5, LOW(), 5);
+
+		assert enrolmentStation.users == {userHigh1, userHigh2, userMedium3, userMedium4, userLow5};
+		assert userLow5.token.clearanceLevel == LOW();
+		assert userLow5.token.fingerprint == 5;
+		assert userLow5.token.valid;
+
+		enrolmentStation.Enrol(userLow6, LOW(), 6);
+
+		assert enrolmentStation.users == {userHigh1, userHigh2, userMedium3, userMedium4, userLow5, userLow6};
+		assert userLow6.token.clearanceLevel == LOW();
+		assert userLow6.token.fingerprint == 6;
+		assert userLow6.token.valid;
+
+
+
+		// ******** Enter door tests ********
+
+		// ***Valid fingerprints***
+		
+		// High security door
+		var accessGranted := doorHigh.EnterDoor(userHigh1, 1);
+		assert userHigh1.token.valid;
+		assert accessGranted;
+
+		accessGranted := doorHigh.EnterDoor(userMedium3, 3);
+		assert userMedium3.token.valid;
+		assert !accessGranted;
+
+		accessGranted := doorHigh.EnterDoor(userLow5, 5);
+		assert userLow5.token.valid;
+		assert !accessGranted;
+
+		// Medium security door
+
+		accessGranted := doorMedium.EnterDoor(userHigh1, 1);
+		assert userHigh1.token.valid;
+		assert accessGranted;
+
+		accessGranted := doorMedium.EnterDoor(userMedium3, 3);
+		assert userMedium3.token.valid;
+		assert accessGranted;
+
+		accessGranted := doorMedium.EnterDoor(userLow5, 5);
+		assert userLow5.token.valid;
+		assert !accessGranted;
+
+		// Low security door
+
+		accessGranted := doorLow.EnterDoor(userHigh1, 1);
+		assert userHigh1.token.valid;
+		assert accessGranted;
+
+		accessGranted := doorLow.EnterDoor(userMedium3, 3);
+		assert userMedium3.token.valid;
+		assert accessGranted;
+
+		accessGranted := doorLow.EnterDoor(userLow5, 5);
+		assert userLow5.token.valid;
+		assert accessGranted;
+
+
+
+		// ***Invalid fingerprints***
+		
+		// High security door
+		accessGranted := doorHigh.EnterDoor(userHigh2, 1);
+		assert !userHigh2.token.valid;
+		assert !accessGranted;
+
+		accessGranted := doorHigh.EnterDoor(userMedium4, 3);
+		assert !userMedium4.token.valid;
+		assert !accessGranted;
+
+		accessGranted := doorHigh.EnterDoor(userLow6, 5);
+		assert !userLow6.token.valid;
+		assert !accessGranted;
+
+		// Medium security door
+
+		accessGranted := doorMedium.EnterDoor(userHigh2, 1);
+		assert !userHigh2.token.valid;
+		assert !accessGranted;
+
+		accessGranted := doorMedium.EnterDoor(userMedium4, 3);
+		assert !userMedium4.token.valid;
+		assert !accessGranted;
+
+		accessGranted := doorMedium.EnterDoor(userLow6, 5);
+		assert !userLow6.token.valid;
+		assert !accessGranted;
+
+		// Low security door
+
+		accessGranted := doorLow.EnterDoor(userHigh2, 1);
+		assert !userHigh2.token.valid;
+		assert !accessGranted;
+
+		accessGranted := doorLow.EnterDoor(userMedium4, 3);
+		assert !userMedium4.token.valid;
+		assert !accessGranted;
+
+		accessGranted := doorLow.EnterDoor(userLow6, 5);
+		assert !userLow6.token.valid;
+		assert !accessGranted;
 }
